src/program_proof/rsm/distx/invariance/linearize.v
@@ -1,0 +1,395 @@
+From Perennial.program_proof.rsm.distx Require Import prelude.
+
+Lemma conflict_past_inv_linearize {past future tmodas} ts form :
+  conflict_cases past future ts form ->
+  conflict_past past future tmodas ->
+  conflict_past past future (<[ts := form]> tmodas).
+Proof. intros Hc Hcp. by apply map_Forall_insert_2. Qed.
+
+Section inv.
+  Context `{!distx_ghostG Σ}.
+
+  Definition key_inv_linearizable_after γ (key : dbkey) (ts : nat) : iProp Σ :=
+    ∃ tslb, key_inv_with_tslb γ key tslb ∗ ⌜(tslb ≤ ts)%nat⌝.
+
+  Definition key_inv_no_kmodl_linearizable_after
+    γ (key : dbkey) (kmodl : dbkmod) (ts : nat) : iProp Σ :=
+    ∃ tslb, key_inv_with_tslb_no_kmodl γ key tslb kmodl ∗ ⌜(tslb ≤ ts)%nat⌝.
+
+  Lemma keys_inv_before_linearize γ ts keys :
+    ([∗ set] key ∈ keys, key_inv γ key) -∗
+    ts_auth γ ts -∗
+    ([∗ set] key ∈ keys, key_inv_linearizable_after γ key ts) ∗
+    ts_auth γ ts.
+  Proof.
+    iIntros "Hkeys Hts".
+    iApply (big_sepS_impl_res with "Hkeys Hts").
+    iIntros (k Hk) "!> Hkey Hts".
+    iNamed "Hkey".
+    iDestruct (ts_le with "Htslb Hts") as %Hle.
+    iFrame "∗ # %".
+  Qed.
+
+  Lemma keys_inv_after_linearize γ ts keys :
+    ([∗ set] key ∈ keys, key_inv_linearizable_after γ key ts) -∗
+    ([∗ set] key ∈ keys, key_inv γ key).
+  Proof.
+    iIntros "Hkeys".
+    iApply (big_sepS_mono with "Hkeys").
+    iIntros (k Hk) "Hkey".
+    iDestruct "Hkey" as (tslb) "[Hkey %Htslb]".
+    do 2 iNamed "Hkey".
+    iFrame "∗ #".
+  Qed.
+
+  Lemma keys_inv_witness_hist_lnrz_at γ ts tid rds :
+    (ts < tid)%nat ->
+    ts_lb γ tid -∗
+    db_ptstos γ rds -∗
+    ([∗ set] key ∈ dom rds, key_inv_linearizable_after γ key ts) ==∗
+    db_ptstos γ rds ∗
+    ([∗ set] key ∈ dom rds, key_inv_linearizable_after γ key (pred tid)) ∗
+    ([∗ map] key ↦ value ∈ rds, hist_lnrz_at γ key (pred tid) value).
+  Proof.
+    iIntros (Htid) "#Htid Hpts Hkeys".
+    rewrite 2!big_sepS_big_sepM -big_sepM_sep /db_ptstos.
+    iCombine "Hpts Hkeys" as "Hptskeys".
+    rewrite -2!big_sepM_sep -big_sepM_bupd.
+    iApply (big_sepM_impl with "Hptskeys").
+    iIntros (k v Hv) "!> [Hpt Hkey]".
+    iDestruct "Hkey" as (tslb) "[Hkey %Htslb]".
+    do 2 iNamed "Hkey". iNamed "Hprop".
+    iDestruct (db_ptsto_agree with "Hpt Hdbv") as %->.
+    (* Re-establish [ext_by_lnrz]. *)
+    pose proof (ext_by_lnrz_inv_linearize_abort tid _ _ _ Hdiffl) as Hdiffl'.
+    set lnrz' := last_extend _ _ in Hdiffl'.
+    (* Update [hist_lnrz_auth]. *)
+    iMod (hist_lnrz_update lnrz' with "Hlnrz") as "Hlnrz".
+    { apply last_extend_prefix. }
+    (* Extract a witness that the value of linearized history at [pred tid] is [v]. *)
+    iAssert (hist_lnrz_at γ k (pred tid) v)%I as "#Hlb".
+    { iDestruct (hist_lnrz_witness with "Hlnrz") as "#Hlb".
+      iFrame "Hlb".
+      iPureIntro.
+      rewrite lookup_last_extend_r.
+      { apply Hlast. }
+      { lia. }
+      { lia. }
+    }
+    (* Weaken the new [ts_lb] and clear the unneeded one. *)
+    iDestruct (ts_lb_weaken (pred tid) with "Htid") as "Htid'"; first lia.
+    iClear "Htslb Htid".
+    iFrame "∗ # %".
+    iPureIntro.
+    split; last done.
+    split.
+    { by rewrite last_last_extend. }
+    { rewrite last_extend_length; last first.
+      { intros Hnil. by subst lnrz. }
+      lia.
+    }
+  Qed.
+
+  Lemma keys_inv_linearize_commit {γ kmodls rds} wrs ts tid :
+    (ts < tid)%nat ->
+    dom wrs = dom rds ->
+    dom kmodls = dom wrs ->
+    ts_lb γ tid -∗
+    db_ptstos γ rds -∗
+    ([∗ map] key ↦ kmodl ∈ kmodls,
+       key_inv_no_kmodl_linearizable_after γ key kmodl ts) ==∗
+    db_ptstos γ wrs ∗
+    ([∗ map] key ↦ kmodl;v ∈ kmodls;wrs,
+       key_inv_no_kmodl γ key (<[tid := v]> kmodl)).
+  Proof.
+    iIntros (Htid Hdomwrs Hdomkmodls) "#Htid Hpts Hkeys".
+    iCombine "Hpts Hkeys" as "Hptskeys".
+    rewrite -big_sepM2_sepM; last first.
+    { intros k. rewrite -2!elem_of_dom. set_solver. }
+    rewrite /db_ptstos.
+    rewrite (big_sepM_big_sepM2 _ _ kmodls); last apply Hdomkmodls.
+    rewrite (big_sepM2_flip _ wrs kmodls) -big_sepM2_sep -big_sepM2_bupd.
+    iApply (big_sepM2_impl_dom_eq with "Hptskeys"); [set_solver | set_solver |].
+    iIntros (k x kmodl y kmodl' Hx Hkmodl Hy Hkmodl') "!> [Hpt Hkey]".
+    rewrite Hkmodl in Hkmodl'. symmetry in Hkmodl'. inv Hkmodl'.
+    iDestruct "Hkey" as (tslb) "[Hkey %Htslb]".
+    iNamed "Hkey". iNamed "Hprop".
+    (* Re-establish [ext_by_lnrz]. *)
+    unshelve epose proof (ext_by_lnrz_inv_linearize_commit tid y _ _ _ _ Hdiffl) as Hdiffl'.
+    { (* solved with [Htid, Htslb, Hext] *) lia. }
+    set lnrz' := _ ++ _ in Hdiffl'.
+    (* Update [hist_lnrz_auth]. *)
+    iMod (hist_lnrz_update lnrz' with "Hlnrz") as "Hlnrz".
+    { apply prefix_app_r, last_extend_prefix. }
+    iMod (db_ptsto_update y with "Hpt Hdbv") as "[Hpt Hdbv]".
+    iClear "Htslb".
+    iFrame "∗ # %".
+    iPureIntro.
+    split; first by rewrite last_snoc.
+    rewrite length_app /=.
+    rewrite last_extend_length_eq_n; last first.
+    { lia. }
+    { intros Hnil. by subst lnrz. }
+    lia.
+  Qed.
+
+  Lemma txn_inv_linearize_abort γ (Q : dbmap -> dbmap -> Prop) ts tid future rds form :
+    let Qr := λ wrs, Q rds wrs ∧ dom wrs ⊆ dom rds in
+    dom rds ⊆ keys_all ->
+    (ts < tid)%nat ->
+    conflict_cases [] future tid form ->
+    ts_lb γ tid -∗
+    incorrect_fcc γ tid form -∗
+    db_ptstos γ rds -∗
+    txn_inv_with_future_no_ts γ future ts -∗
+    ([∗ set] key ∈ keys_all, key_inv_linearizable_after γ key ts) ==∗
+    db_ptstos γ rds ∗
+    txn_inv_with_future_no_ts γ future tid ∗
+    ([∗ set] key ∈ keys_all, key_inv γ key) ∗
+    txnpost_receipt γ tid Qr ∗
+    ([∗ map] key ↦ value ∈ rds, hist_lnrz_at γ key (pred tid) value) ∗
+    txns_lnrz_receipt γ tid.
+  Proof.
+    iIntros (Qr Hdomrds Hts Hcft) "#Htslb #Hfcc Hpts Htxn Hkeys".
+    iNamed "Htxn".
+    (* Obtain [dom rds] of [hist_lnrz_at]. *)
+    iDestruct (big_sepS_subseteq_difference_1 _ _ (dom rds) with "Hkeys") as "[Hkeys HkeysO]".
+    { apply Hdomrds. }
+    iMod (keys_inv_witness_hist_lnrz_at with "Htslb Hpts Hkeys") as "(Hpts & Hkeys & #Hlbs)".
+    { apply Hts. }
+    (* Put [dom rds] of [key_inv]. *)
+    iDestruct (keys_inv_after_linearize with "Hkeys") as "Hkeys".
+    iDestruct (keys_inv_after_linearize with "HkeysO") as "HkeysO".
+    iDestruct (big_sepS_subseteq_difference_2 with "Hkeys HkeysO") as "Hkeys".
+    { apply Hdomrds. }
+    (* Update [txns_lnrz_auth] and obtain a witness that [tid] has linearized. *)
+    iMod (txns_lnrz_insert _ _ tid with "Htxnsl") as "[Htxnsl #Hlnrzed]".
+    { intros Hin. specialize (Htsge _ Hin). simpl in Htsge. lia. }
+    (* Update [tids_excl_auth]. *)
+    iMod (tids_excl_insert _ _ tid with "Hexcl") as "[Hexcl Hexcltid]".
+    { intros Hin. specialize (Htsge _ Hin). simpl in Htsge. lia. }
+    (* Update [txnpost_auth] and obtain a witness. *)
+    iMod (txnpost_insert _ _ tid Qr with "Hpost") as "[Hpost #Htp]".
+    { rewrite -not_elem_of_dom Hdomq. intros Hin. specialize (Htsge _ Hin). simpl in Htsge. lia. }
+    (* Re-establish [ge_all ts ({[tid]} ∪ tids)]. *)
+    assert (Htsge' : ge_all tid ({[tid]} ∪ tids)).
+    { apply set_Forall_union; first by rewrite set_Forall_singleton.
+      intros tidx Htidx.
+      specialize (Htsge _ Htidx). simpl in Htsge.
+      lia.
+    }
+    destruct form as [| wrs | wrs]; simpl in Hcft.
+    { (* Case: No commit in the entire list of actions. *)
+      (* Add [(tid, NC)] to [tmodas]. *)
+      iAssert (partitioned_tids γ ({[tid]} ∪ tids) tmodcs (<[tid := NC]> tmodas) resm)%I
+        with "[Hpart Hexcltid]" as "Hpart".
+      { iNamed "Hpart".
+        iDestruct (big_sepS_insert_2 with "Hexcltid Hwabts") as "Hwabts".
+        rewrite /partitioned_tids dom_insert_L.
+        iFrame.
+        iPureIntro.
+        set_solver.
+      }
+      unshelve epose proof (conflict_past_inv_linearize tid NC Hcft Hcp) as Hcp'.
+      iFrame "∗ # %".
+      iModIntro.
+      iSplit.
+      { by iApply big_sepM_insert_2. }
+      by rewrite dom_insert_L Hdomq.
+    }
+    { (* Case: First commit incompatible with some previous actions. *)
+      iAssert (partitioned_tids γ ({[tid]} ∪ tids) tmodcs (<[tid := FCI wrs]> tmodas) resm)%I
+        with "[Hpart Hexcltid]" as "Hpart".
+      { iNamed "Hpart".
+        iDestruct (big_sepS_insert_2 with "Hexcltid Hwabts") as "Hwabts".
+        rewrite /partitioned_tids dom_insert_L.
+        iFrame.
+        iPureIntro.
+        set_solver.
+      }
+      unshelve epose proof (conflict_past_inv_linearize tid (FCI wrs) _ Hcp) as Hcp'.
+      { destruct Hcft as (lp & ls & Hfc & Hincomp). simpl in Hincomp.
+        exists lp, ls.
+        split; first apply Hfc.
+        rewrite /incompatible_exists Exists_exists in Hincomp.
+        destruct Hincomp as (a & Halp & Hincomp).
+        rewrite /incompatible_exists Exists_exists.
+        exists a.
+        split; [set_solver | done].
+      }
+      iFrame "∗ # %".
+      iModIntro.
+      iSplit.
+      { by iApply big_sepM_insert_2. }
+      by rewrite dom_insert_L Hdomq.
+    }
+    { (* Case: [Q rds wrs] does not hold. *)
+      iAssert (partitioned_tids γ ({[tid]} ∪ tids) tmodcs (<[tid := FCC wrs]> tmodas) resm)%I
+        with "[Hpart Hexcltid]" as "Hpart".
+      { iNamed "Hpart".
+        iDestruct (big_sepS_insert_2 with "Hexcltid Hwabts") as "Hwabts".
+        rewrite /partitioned_tids dom_insert_L.
+        iFrame.
+        iPureIntro.
+        set_solver.
+      }
+      unshelve epose proof (conflict_past_inv_linearize tid (FCC wrs) Hcft Hcp) as Hcp'.
+      iFrame "∗ # %".
+      iModIntro.
+      iSplit.
+      { by iApply big_sepM_insert_2. }
+      by rewrite dom_insert_L Hdomq.
+    }
+  Qed.
+
+  (* Do this at linearization point:
+     destruct (decide (Q rds wrs ∧ dom wrs ⊆ dom rds)) as [[_ Hdomwrs] | Hneg]; last first.
+   *)
+
+  Lemma txn_inv_linearize_commit γ (Q : dbmap -> dbmap -> Prop) ts tid future rds wrs :
+    let Qr := λ wrs, Q rds wrs ∧ dom wrs ⊆ dom rds in
+    dom wrs ⊆ dom rds ->
+    dom rds ⊆ keys_all ->
+    (ts < tid)%nat ->
+    first_commit_compatible future tid wrs ->
+    ts_lb γ tid -∗
+    db_ptstos γ rds -∗
+    txn_inv_with_future_no_ts γ future ts -∗
+    ([∗ set] key ∈ keys_all, key_inv_linearizable_after γ key ts) ==∗
+    db_ptstos γ (wrs ∪ rds) ∗
+    txn_inv_with_future_no_ts γ future tid ∗
+    ([∗ set] key ∈ keys_all, key_inv γ key) ∗
+    txnpost_receipt γ tid Qr ∗
+    ([∗ map] key ↦ value ∈ rds, hist_lnrz_at γ key (pred tid) value) ∗
+    txns_lnrz_receipt γ tid.
+  Proof.
+    iIntros (Qr Hdomwrs Hdomrds Hts Hfcc) "#Htslb Hpts Htxn Hkeys".
+    iNamed "Htxn".
+    (* Obtain [dom rds] of [hist_lnrz_at]. *)
+    iDestruct (big_sepS_subseteq_difference_1 _ _ (dom rds) with "Hkeys") as "[Hkeys HkeysO]".
+    { apply Hdomrds. }
+    iMod (keys_inv_witness_hist_lnrz_at with "Htslb Hpts Hkeys") as "(Hpts & Hkeys & #Hlbs)".
+    { apply Hts. }
+    (* Update [txns_lnrz_auth] and obtain a witness that [tid] has linearized. *)
+    iMod (txns_lnrz_insert _ _ tid with "Htxnsl") as "[Htxnsl #Hlnrzed]".
+    { intros Hin. specialize (Htsge _ Hin). simpl in Htsge. lia. }
+    (* Update [tids_excl_auth]. *)
+    iMod (tids_excl_insert _ _ tid with "Hexcl") as "[Hexcl Hexcltid]".
+    { intros Hin. specialize (Htsge _ Hin). simpl in Htsge. lia. }
+    (* Prove [tmodcs !! tid = None]. *)
+    iAssert (⌜tmodcs !! tid = None⌝)%I as %Hnotintmodcs.
+    { iNamed "Hpart".
+      iDestruct (tids_excl_not_elem_of with "Hwcmts Hexcltid") as %Hnotin.
+      by rewrite not_elem_of_dom in Hnotin.
+    }
+    (* Update [txnpost_auth] and obtain a witness. *)
+    iMod (txnpost_insert _ _ tid Qr with "Hpost") as "[Hpost #Htp]".
+    { rewrite -not_elem_of_dom Hdomq. intros Hin. specialize (Htsge _ Hin). simpl in Htsge. lia. }
+    (* Re-establish [ge_all ts ({[tid]} ∪ tids)]. *)
+    assert (Htsge' : ge_all tid ({[tid]} ∪ tids)).
+    { apply set_Forall_union; first by rewrite set_Forall_singleton.
+      intros tidx Htidx.
+      specialize (Htsge _ Htidx). simpl in Htsge.
+      lia.
+    }
+    (* Obtain [dom wrs] of [kmod_lnrz_half] from the txnsys invariant. *)
+    iDestruct (big_sepS_subseteq_difference_1 _ _ (dom wrs) with "Hkmodls") as "[Hkmodls HkmodlsO]".
+    { set_solver. }
+    (* Obtain [dom wrs] of [kmod_lnrz_half] from the keys invariant. *)
+    iDestruct (big_sepS_subseteq_difference_1 _ _ (dom wrs) with "Hkeys") as "[Hkeys HkeysR]".
+    { set_solver. }
+    (* Extract [kmod_lnrz_half] out of [key_inv_linearizable_after]. *)
+    iDestruct (big_sepS_exists_sepM with "Hkeys") as (tslbm) "[%Hdomtslbm Hkeys]".
+    iDestruct (big_sepM_sep with "Hkeys") as "[Hkeys %Htslbm]".
+    iDestruct (keys_inv_with_tslb_extract_kmodl with "Hkeys") as (kmodls) "[Hkeys Hkmodls']".
+    iDestruct (big_sepM2_dom with "Hkeys") as %Hdomkmodls.
+    (* Agreement of [kmod_lnrz_half] between [txn_inv] and [key_inv]. *)
+    iDestruct (kmod_lnrz_big_agree with "Hkmodls Hkmodls'") as %Hkmodls.
+    { set_solver. }
+    (* Update [kmod_lnrz_half]. *)
+    set tmodcs' := <[tid := wrs]> tmodcs.
+    iMod (kmod_lnrz_big_update (λ k, vslice tmodcs' k) with
+           "Hkmodls Hkmodls'") as "[Hkmodls Hkmodls']".
+    { set_solver. }
+    iAssert ([∗ map] k ↦ kmod;v ∈ kmodls;wrs, kmod_lnrz_half γ k (<[tid := v]> kmod))%I
+      with "[Hkmodls']" as "Hkmodls'".
+    { iApply (big_sepM_sepM2_impl with "Hkmodls'").
+      { set_solver. }
+      iIntros (k kmod v Hkmod Hv) "!> Hkmods".
+      subst tmodcs'.
+      specialize (Hkmodls _ _ Hkmod).
+      by rewrite (vslice_insert_Some _ _ _ _ _ Hv) Hkmodls.
+    }
+    (* Update the unmodified part of [kmod_lnrz_half] (from [txn_inv]). *)
+    iAssert ([∗ set] x ∈ (keys_all ∖ dom wrs), kmod_lnrz_half γ x (vslice tmodcs' x))%I
+      with "[HkmodlsO]" as "HkmodlsO".
+    { iApply (big_sepS_impl with "HkmodlsO").
+      iIntros (k Hk) "!> Hkmod".
+      subst tmodcs'.
+      assert (Hnotinwrs : wrs !! k = None).
+      { rewrite -not_elem_of_dom. set_solver. }
+      by rewrite (vslice_insert_None _ _ _ _ Hnotintmodcs Hnotinwrs).
+    }
+    (* Combine modified and unmodified parts of [kmod_lnrz_half]. *)
+    iDestruct (big_sepS_subseteq_difference_2 with "Hkmodls HkmodlsO") as "Hkmodls".
+    { set_solver. }
+    (* Re-retablish [key_inv_linearizable_after] w.r.t. linearize-commit. *)
+    iAssert ([∗ map] k ↦ kmodl ∈ kmodls, key_inv_no_kmodl_linearizable_after γ k kmodl (pred tid))%I
+      with "[Hkeys]" as "Hkeys".
+    { iApply (big_sepM2_sepM_impl with "Hkeys"); first set_solver.
+      iIntros (k tslb kmod kmod' Htslb Hkmod Hkmod') "!> Hkey".
+      rewrite Hkmod in Hkmod'. symmetry in Hkmod'. inv Hkmod'.
+      specialize (Htslbm _ _ Htslb). simpl in Htslbm.
+      iFrame "∗ %".
+    }
+    iDestruct (big_sepM_subseteq_difference_1 _ (rds ∩ wrs) with "Hpts") as "[Hpts HptsO]".
+    { apply map_intersection_subseteq. }
+    iMod (keys_inv_linearize_commit wrs _ tid with "Htslb Hpts Hkeys") as "[Hpts Hkeys]".
+    { lia. }
+    { set_solver. }
+    { set_solver. }
+    iCombine "Hpts HptsO" as "Hpts".
+    rewrite -big_sepM_union; last first.
+    { apply map_disjoint_difference_union. }
+    rewrite map_intersection_difference_union.
+    (* Put [kmod_lnrz_half] back to [key_inv_linearizable_after]. *)
+    iAssert ([∗ set] k ∈ dom wrs, key_inv γ k)%I with "[Hkeys Hkmodls']" as "Hkeys".
+    { iCombine "Hkeys Hkmodls'" as "Hkeys".
+      rewrite -big_sepM2_sep.
+      rewrite big_sepS_big_sepM.
+      iApply (big_sepM2_sepM_impl with "Hkeys"); first set_solver.
+      iIntros (k kmodl v v' Hkmodl Hv _) "!> Hkey". clear v'.
+      iDestruct "Hkey" as "[Hkey Hkmodl]".
+      do 2 (iNamed "Hkey").
+      iFrame "∗ # %".
+    }
+    iDestruct (keys_inv_after_linearize with "HkeysR") as "HkeysR".
+    iDestruct (big_sepS_subseteq_difference_2 with "Hkeys HkeysR") as "Hkeys".
+    { apply Hdomwrs. }
+    (* Re-establish [paritioned_tids]. *)
+    iAssert (partitioned_tids γ ({[tid]} ∪ tids) (<[tid := wrs]> tmodcs) tmodas resm)%I
+      with "[Hpart Hexcltid]" as "Hpart".
+    { iNamed "Hpart".
+      iDestruct (big_sepS_insert_2 with "Hexcltid Hwcmts") as "Hwcmts".
+      rewrite /partitioned_tids dom_insert_L.
+      iFrame.
+      iPureIntro.
+      set_solver.
+    }
+    iDestruct (keys_inv_after_linearize with "HkeysO") as "HkeysO".
+    iDestruct (big_sepS_subseteq_difference_2 with "Hkeys HkeysO") as "Hkeys".
+    { apply Hdomrds. }
+    iFrame "∗ # %".
+    iPureIntro.
+    split; first by rewrite dom_insert_L Hdomq.
+    split.
+    { rewrite dom_insert_L.
+      apply set_Forall_union; last apply Hnz.
+      rewrite set_Forall_singleton.
+      (* solved with [Hts]. *)
+      lia.
+    }
+    { by apply map_Forall_insert_2. }
+  Qed.
+
+End inv.
